CSS/Semantics.v
@@ -5,7 +5,7 @@ Require Import Coq.Bool.Bool.
 Import ListNotations.
 Open Scope string_scope.
 
-(** 1. REFINED AST & SELECTORS *)
+(** 1. AST & SELECTORS *)
 
 Inductive Tag : Set := div | span | p | img | h1.
 
@@ -23,7 +23,8 @@ Inductive Node : Set :=
 
 Inductive Property : Set :=
   | p_width | p_height | p_margin | p_padding | p_border
-  | p_color | p_display | p_box_sizing.
+  | p_color | p_display | p_box_sizing
+  | p_position | p_top | p_left | p_z_index.
 
 Inductive Value : Set :=
   | v_px : nat -> Value
@@ -39,13 +40,12 @@ Inductive Selector : Set :=
   | sel_tag   : Tag -> Selector
   | sel_class : string -> Selector
   | sel_id    : string -> Selector
-  | sel_desc  : Selector -> Selector -> Selector. (* Descendant: s1 s2 *)
+  | sel_desc  : Selector -> Selector -> Selector.
 
 Record Rule : Set := { rule_sel : Selector; rule_decls : list Decl }.
-
 Definition CSS := list Rule.
 
-(** 2. ADVANCED CASCADE (Specificity + !important + Descendants) *)
+(** 2. CASCADE *)
 
 Fixpoint specificity (s : Selector) : nat :=
   match s with
@@ -61,7 +61,6 @@ Fixpoint find_attr (name : string) (attrs : list Attr) : option string :=
   | a :: as' => if (attr_name a =? name)%string then Some (attr_value a) else find_attr name as'
   end.
 
-(* Matches now needs ancestors for descendant selectors *)
 Fixpoint matches (ancestors : list Node) (n : Node) (s : Selector) : bool :=
   match s with
   | sel_tag t' => match n with elem t _ _ => tag_eq t t' | _ => false end
@@ -73,7 +72,7 @@ Fixpoint matches (ancestors : list Node) (n : Node) (s : Selector) : bool :=
                       | _ => false end
   | sel_desc s1 s2 => 
       if matches ancestors n s2 then
-        existsb (fun anc => matches [] anc s1) ancestors (* Simplified: check any ancestor *)
+        existsb (fun anc => matches [] anc s1) ancestors
       else false
   end.
 
@@ -81,7 +80,9 @@ Definition prop_eq (p1 p2 : Property) : bool :=
   match p1, p2 with
   | p_width, p_width => true | p_height, p_height => true | p_margin, p_margin => true
   | p_padding, p_padding => true | p_border, p_border => true | p_color, p_color => true 
-  | p_display, p_display => true | p_box_sizing, p_box_sizing => true | _, _ => false
+  | p_display, p_display => true | p_box_sizing, p_box_sizing => true 
+  | p_position, p_position => true | p_top, p_top => true | p_left, p_left => true
+  | p_z_index, p_z_index => true | _, _ => false
   end.
 
 Fixpoint find_decl (p : Property) (decls : list Decl) : option Decl :=
@@ -90,7 +91,6 @@ Fixpoint find_decl (p : Property) (decls : list Decl) : option Decl :=
   | d :: ds => if prop_eq p (decl_prop d) then Some d else find_decl p ds
   end.
 
-(** Cascade resolution with !important and specificity *)
 Fixpoint cascade_resolve (anc : list Node) (p : Property) (n : Node) (css : CSS) 
                          (best_spec : nat) (best_imp : bool) (best_val : option Value) : option Value :=
   match css with
@@ -101,7 +101,6 @@ Fixpoint cascade_resolve (anc : list Node) (p : Property) (n : Node) (css : CSS)
         | Some d => 
             let spec := specificity (rule_sel r) in
             let imp := decl_important d in
-            (* !important always wins over normal; then specificity *)
             if (orb (andb imp (negb best_imp)) (andb (eqb imp best_imp) (leb best_spec spec)))
             then cascade_resolve anc p n rs spec imp (Some (decl_val d))
             else cascade_resolve anc p n rs best_spec best_imp best_val
@@ -113,18 +112,19 @@ Fixpoint cascade_resolve (anc : list Node) (p : Property) (n : Node) (css : CSS)
 Definition resolve (anc : list Node) (p : Property) (n : Node) (css : CSS) : option Value :=
   cascade_resolve anc p n css 0 false None.
 
-(** 3. FULL BOX MODEL STYLE *)
+(** 3. POSITIONING & STYLE *)
 
+Inductive Position : Set := s_static | s_relative | s_absolute.
 Record SideValues : Set := { t_v : nat; r_v : nat; b_v : nat; l_v : nat }.
 Inductive BoxSizing : Set := content_box | border_box.
 Inductive DisplayType : Set := d_block | d_inline | d_none.
 
 Record Style : Set := {
   s_disp : DisplayType;
+  s_pos : Position;
+  s_top : nat; s_left : nat; s_z_index : nat;
   s_width : nat; s_height : nat;
-  s_margin : SideValues;
-  s_padding : SideValues;
-  s_border : SideValues;
+  s_margin : SideValues; s_padding : SideValues; s_border : SideValues;
   s_box_sizing : BoxSizing;
   s_color : string
 }.
@@ -136,7 +136,16 @@ Definition compute_style (anc : list Node) (parent : option Style) (n : Node) (c
               | Some (v_str "none") => d_none
               | _ => d_block
               end in
+  let pos := match resolve anc p_position n css with
+             | Some (v_str "relative") => s_relative
+             | Some (v_str "absolute") => s_absolute
+             | _ => s_static
+             end in
   {| s_disp := disp;
+     s_pos := pos;
+     s_top := get_px p_top 0;
+     s_left := get_px p_left 0;
+     s_z_index := get_px p_z_index 0;
      s_width := get_px p_width 0;
      s_height := get_px p_height 0;
      s_margin := let v := get_px p_margin 0 in {| t_v := v; r_v := v; b_v := v; l_v := v |};
@@ -148,13 +157,12 @@ Definition compute_style (anc : list Node) (parent : option Style) (n : Node) (c
                 | Some (v_str c) => c 
                 | _ => match parent with Some ps => s_color ps | None => "black" end end |}.
 
-(** 4. VISUAL FORMATTING MODEL (Layout) *)
+(** 4. LAYOUT WITH POSITIONING *)
 
 Record Rect : Set := { rx : nat; ry : nat; rw : nat; rh : nat }.
 Inductive Box : Set := mkBox : Node -> Rect -> Style -> list Box -> Box.
 Definition Layout := list Box.
 
-(* Layout now tracks horizontal offset for inline elements *)
 Definition layout_node (anc : list Node) (availW : nat) (parent_s : option Style) 
                      (x y : nat) (n : Node) (css : CSS) : (list Box * nat * nat) :=
   let s := compute_style anc parent_s n css in
@@ -165,8 +173,16 @@ Definition layout_node (anc : list Node) (availW : nat) (parent_s : option Style
       let p := s_padding s in
       let b := s_border s in
       
-      let bx := x + l_v m in
-      let by := y + t_v m in
+      let flow_x := x + l_v m in
+      let flow_y := y + t_v m in
+      
+      let final_pos := match s_pos s with
+                       | s_relative => (flow_x + s_left s, flow_y + s_top s)
+                       | s_absolute => (s_left s, s_top s)
+                       | s_static => (flow_x, flow_y)
+                       end in
+      let fx := fst final_pos in
+      let fy := snd final_pos in
       
       let content_w := if Nat.eqb (s_width s) 0 then 50 else s_width s in
       let content_h := if Nat.eqb (s_height s) 0 then 20 else s_height s in
@@ -180,18 +196,18 @@ Definition layout_node (anc : list Node) (availW : nat) (parent_s : option Style
                   | border_box => content_h
                   end in
                   
-      let box := mkBox n (Build_Rect bx by bb_w bb_h) s [] in
+      let box := mkBox n (Build_Rect fx fy bb_w bb_h) s [] in
       
       match s_disp s with
       | d_block => ([box], x, y + bb_h + t_v m + b_v m)
       | d_inline => ([box], x + bb_w + l_v m + r_v m, y)
+      | d_none => ([], x, y)
       end
   end.
 
 Definition render (availW : nat) (n : Node) (css : CSS) : Layout :=
-  let res := layout_node [] availW None 0 0 n css in
-  match res with
-  | (boxes, _, _) => boxes
+  match (layout_node [] availW None 0 0 n css) with
+  | (res, _, _) => res
   end.
 
 (** 5. VERIFICATION *)
@@ -199,25 +215,14 @@ Definition render (availW : nat) (n : Node) (css : CSS) : Layout :=
 Theorem render_unique : forall w n css o1 o2, render w n css = o1 -> render w n css = o2 -> o1 = o2.
 Proof. intros. rewrite <- H, <- H0. reflexivity. Qed.
 
-(* Test: !important override *)
-Example test_important :
+(* Test: Absolute Positioning *)
+Example test_absolute :
   let css := [ {| rule_sel := sel_tag div ; 
-                  rule_decls := [ {| decl_prop := p_color ; decl_val := v_str "red" ; decl_important := true |} ] |} ;
-               {| rule_sel := sel_id "myid" ; 
-                  rule_decls := [ {| decl_prop := p_color ; decl_val := v_str "blue" ; decl_important := false |} ] |} ] in
-  let n := elem div [ {| attr_name := "id" ; attr_value := "myid" |} ] [] in
-  match render 800 n css with
-  | [mkBox _ _ s _] => s_color s = "red"
+                  rule_decls := [ {| decl_prop := p_position ; decl_val := v_str "absolute" ; decl_important := false |} ;
+                                  {| decl_prop := p_top ; decl_val := v_px 50 ; decl_important := false |} ;
+                                  {| decl_prop := p_left ; decl_val := v_px 100 ; decl_important := false |} ] |} ] in
+  match render 800 (elem div [] []) css with
+  | [mkBox _ r _ _] => rx r = 100 /\ ry r = 50
   | _ => False
   end.
-Proof. simpl. reflexivity. Qed.
-
-(* Test: Descendant Selector (div p) *)
-Example test_descendant :
-  let css := [ {| rule_sel := sel_desc (sel_tag div) (sel_tag p) ; 
-                  rule_decls := [ {| decl_prop := p_color ; decl_val := v_str "green" ; decl_important := false |} ] |} ] in
-  let parent := elem div [] [] in
-  let child := elem p [] [] in
-  let s := compute_style [parent] None child css in
-  s_color s = "green".
-Proof. simpl. reflexivity. Qed.
+Proof. simpl. split; reflexivity. Qed.
